hist_bind_resexn_weaken was too optimistic

rupicola/io/RunningExample.fst
@@ -148,8 +148,8 @@ let hist_bind_commut_resexn #a #b (m : hist (resexn a)) (k : a -> io (resexn b))
   lem_hist_bind_equiv m m (fun (r : resexn a) -> theta (match r with | Inl x -> k x | Inr x -> io_return (Inr x))) (fun r -> match r with | Inl x -> theta (k x) | Inr x -> hist_return (Inr x))
 
 let hist_inl #a #b (k : a -> hist (resexn b)) (r : resexn a) : hist (resexn b) =
-  fun h lt ->
-    Inl? r ==> k (Inl?.v r) h lt
+  fun h p ->
+    Inl? r ==> k (Inl?.v r) h p
 
 let hist_bind_resexn_weaken #a #b (m : hist (resexn a)) (k : a -> io (resexn b)) :
   Lemma (
@@ -160,7 +160,22 @@ let hist_bind_resexn_weaken #a #b (m : hist (resexn a)) (k : a -> io (resexn b))
   with begin
     match r with
     | Inl x -> ()
-    | Inr x -> admit ()
+    | Inr x ->
+      // assume (theta (io_return (Inr x)) ⊑ (hist_inl (fun x -> theta (k x))) (Inr x))
+      theta_monad_morphism_ret #(resexn b) (Inr x) ;
+      // assume (hist_return (Inr x) ⊑ (hist_inl (fun x -> theta (k x))) (Inr x))
+      introduce forall h p. (hist_inl (fun x -> theta (k x))) (Inr x) h p ==> hist_return (Inr x) h p
+      with begin
+        // assume ((hist_inl (fun x -> theta (k x))) (Inr x) h p ==> p [] (Inr x))
+        calc (==>) {
+          (hist_inl (fun x -> theta (k x))) (Inr x) h p ;
+          // ^^ this is just a trivial pre
+          ==> { admit () }
+          p [] (Inr x) ;
+          == {}
+          hist_return (Inr x) h p ;
+        }
+      end
   end ;
   lem_hist_bind_subset m m (fun (r : resexn a) -> theta (match r with | Inl x -> k x | Inr x -> io_return (Inr x))) (hist_inl (fun x -> theta (k x)))
 
